theories/tests/heap_lang.v
@@ -86,5 +86,5 @@ Section LiftingTests.
   Proof. iIntros "". wp_apply Pred_spec. wp_let. by wp_apply Pred_spec. Qed.
 End LiftingTests.
 
-Lemma heap_e_adequate σ : adequate true heap_e σ (= #2).
+Lemma heap_e_adequate σ : adequate progress heap_e σ (= #2).
 Proof. eapply (heap_adequacy heapΣ)=> ?. by apply heap_e_spec. Qed.
